\subsection{Formules}
\label{sec:GonioFormules}

\paragraph{Hoofdeigenschap en afleidingen}
\label{sec:HoofdeigenschapGonio}

   \[
	   \sin^2 \alpha + \cos^2 \alpha = 1
   \]
   \[
	   1 + \tan^2 \alpha = \sec^2 \alpha 
   \]
   \[
	   1 + \cot^2 \alpha = \csc^2 \alpha 
   \]
  
\paragraph{Som-- en verschilformules}
\label{sec:SomVerschilfGonio}

   \[
	   \sin( \alpha \pm \beta )  = \sin \alpha \cos \beta \pm \cos \alpha \sin \beta 
   \]
   \[
	   \cos( \alpha \pm \beta )  = \cos \alpha \cos \beta \mp \sin \alpha \sin \beta 
   \]
   \[
	   \tan( \alpha \pm \beta )  = \frac{\tan\alpha \pm \tan \beta}{1 \mp \tan\alpha\tan\beta} 
   \]
  
\paragraph{Verdubbelingsformules}
\label{sec:VerdubbelingsformulesGonio}
   \begin{eqnarray*}
	   \sin 2\alpha & = & 2 \sin \alpha \cdot \cos \alpha\\
	                & = & \frac{2 \tan \alpha }{1 + \tan^2 \alpha}
   \end{eqnarray*}
   \begin{eqnarray*}
	   \cos 2\alpha & = & \cos^2 \alpha - \sin^2 \alpha\\
	                & = & 1 - 2 \sin^2 \alpha\\
	                & = & 2 \cos^2 \alpha - 1\\
	                & = & \frac{1-\tan^2 \alpha}{1+\tan^2 \alpha}
   \end{eqnarray*}
   \begin{eqnarray*}
	   \tan 2\alpha & = & \frac{2 \tan \alpha}{1- \tan^2 \alpha}
   \end{eqnarray*}  
  
\paragraph{t-formules}
\label{sec:tFormulesGonio}

 ( $t = \tan \frac{\alpha}{2} $ )
   \[
	   \sin \alpha = \frac{2t}{1+t^2} 
   \]
   \[
	   \cos \alpha = \frac{1-t^2}{1+t^2} 
   \]
   \[
	   \tan \alpha = \frac{2t}{1-t^2} 
   \]
  
\paragraph{Productformules}
\label{sec:ProductformulesGonio}

   \[
	   \sin 3\alpha = 3 \sin \alpha - 4 \sin^3 \alpha
   \]
   \[
	   \cos 3\alpha = 4 \cos^3 \alpha - 3\cos\alpha 
   \]
   \[
	   \sin^2 \alpha = \frac{1-\cos 2\alpha}{2}
   \]
   \[
	   \cos^2 \alpha = \frac{1+\cos 2\alpha}{2} 
   \]
  \newpage
  
\paragraph{Formules van Simpson (product naar som)}
\label{sec:FormulesVanSimpsonPS}
   \[
	   2\sin\alpha \cdot \cos\beta = \sin ( \alpha + \beta ) + \sin ( \alpha - \beta )
   \]
   \[
	   2\cos\alpha \cdot \cos\beta = \cos ( \alpha + \beta ) + \cos ( \alpha - \beta ) 
   \]
   \[
	   2\sin\alpha \cdot \sin\beta = \cos ( \alpha - \beta ) - \cos ( \alpha + \beta ) 
   \]
   \[
	   2\cos\alpha \cdot \sin\beta = \sin ( \alpha + \beta ) - \sin ( \alpha - \beta ) 
   \]
   
\paragraph{Formules van Simpson (som naar product)}
\label{sec:FormulesVanSimpsonSP}

   \[
	   \sin p + \sin q = 2\sin\frac{p+q}{2}\cos\frac{p-q}{2} 
   \]
   \[
	   \sin p - \sin q = 2\cos\frac{p+q}{2}\sin\frac{p-q}{2} 
   \]
   \[
	   \cos p + \cos q = 2\cos\frac{p+q}{2}\cos\frac{p-q}{2} 
   \]
   \[
	   \cos p - \cos q = -2\sin\frac{p+q}{2}\sin\frac{p-q}{2} 
   \]