\[
  \overrightarrow{AB} = \vec{B} - \vec{A}
\]

\paragraph{Rekenregels}
\label{sec:RekenregelsVectoren}
     \[
       \forall \vec a:
          \vec a \cdot \vec o = 0 = \vec o \cdot \vec a
     \]
   \[
       \forall \vec a \neq \vec o:
          \vec a \cdot \vec a = ||\vec a||^2
     \]
     \[
       \forall \vec a, \vec b :
          \vec a \cdot \vec b = \vec b \cdot \vec a
           \Leftrightarrow \scalprodv{a}{b} = \scalprodv{b}{a}
     \]
     \[
       \forall \vec a, \vec b \neq \vec o:
          \vec a \bot \vec b \Leftrightarrow \vec a \cdot \vec b = 0
     \]

\paragraph{Scalair product}
\label{sec:scalairProduct}
     \[
       \forall \vec u, \vec v \neq \vec o :
          \vec u \cdot \vec v = ||\vec u|| \cdot ||\vec v|| \cdot \cos\left(\widehat{\vec u, \vec v}\right)
                              = \sum_{i=1}^n u_iv_i
     \]
\paragraph{Vectoriëel Product}
\label{sec:VectorieelProduct}
  \[
    \vec a \times \vec b =
    \left|
     \begin{array}{ccc}
       \vec u_x  &  \vec u_y  &  \vec u_z \\
      a_x & a_y & a_z\\
      b_x & b_y & b_z
     \end{array}
   \right|
  \]
\paragraph{Gemengd product}
\label{sec:GemengdProduct}
  \[
    \left(\vec a \times \vec b \right) \cdot \vec c=
    \left|
     \begin{array}{ccc}
      c_x & c_y & c_z \\
      a_x & a_y & a_z\\
      b_x & b_y & b_z
     \end{array}
   \right|
  \]

\paragraph{Lengtes/Normen}
\label{sec:Lengtes}
\[
  \left\| \vec{x} \right\| =
  \left\| \vec{x} \right\|_1 =
  \sqrt{\sum_i^n x_i^2}
  \qquad
  \mbox{Euclidische norm}
\]
\[
  \left\| \vec{x} \right\|_2 =
  \max \left\{ x_1,  \ldots, x_n \right\}
  \qquad
  \mbox{maximumnorm}
\]
\[
  \left\| \vec{x} \right\|_3 =
  \sum_i^n \left| x_i \right|
  \qquad
  \mbox{Chebyshevnorm}
\]

\paragraph{Differentiaaloperatoren}
\label{sec:Differentiaaloperatoren}

\subparagraph{Differentiaaloperator van de Eerste Orde}
\label{sec:Differentiaaloperator1}
  \[
    \vec \nabla = \left(\frac{\partial}{\partial x},\frac{\partial}{\partial y},\frac{\partial}{\partial z}\right)
  \]

\subparagraph{Gradiënt}
\label{sec:Gradient}
  \[
    \mbox{grad}\left(f\right) = \vec \nabla f =  \left(\frac{\partial f}{\partial x},\frac{\partial f}{\partial y},\frac{\partial f}{\partial z}\right)
  \]

\subparagraph{Divergentie}
\label{sec:Divergentie}
  \[
    \mbox{div}\left(\vec v\right) = \vec \nabla \cdot \vec v = \frac{\partial v_x}{\partial x} + \frac{\partial v_y}{\partial y} + \frac{\partial v_z}{\partial z}
  \]

\subparagraph{Rotatie}
\label{sec:Rotatie}
  \[
    \mbox{rot}\left(\vec v\right) = \vec \nabla \times \vec v =
    \left|
     \begin{array}{ccc}
       \vec u_x  &  \vec u_y  &  \vec u_z \\
       \frac{\partial}{\partial x} & \frac{\partial}{\partial y} & \frac{\partial}{\partial z}\\
      v_x & v_y & v_z
     \end{array}
   \right|
  \]

\subparagraph{Differentiaaloperator van de Tweede Orde (Laplaciaan)}
\label{sec:Differentiaaloperator2}
  \[
    \Delta\left(f\right)=\mbox{div}\left(\mbox{grad}\left(f\right)\right)=
    \vec \nabla \cdot\left(\vec \nabla f\right) = \vec \nabla^2 f =
    \frac{\partial^2 f}{\partial x^2} + \frac{\partial^2 f}{\partial y^2} + \frac{\partial^2 f}{\partial z^2}
  \]

\paragraph{Coördinatenstelsels}
\label{sec:CoordStelsels}

\subparagraph{Cartesisch}
\[
  \left\{
    \begin{array}{l}
      x = x\\
      y = y\\
      z = z\\
    \end{array}
  \right.
\]
\[
  \left| J \right| = 1
\]

\subparagraph{Poolcoördinaten/Cilindercoordinaten}
\[
  \left\{
    \begin{array}{l}
      x = r \cos \theta\\
      y = r \sin \theta\\
      z = z\\
    \end{array}
  \right.
\]
\[
  \left| J \right| =
  \left|
    \begin{array}{ccc}
      \cos \theta & - r \sin \theta & 0 \\
      \sin \theta &   r \cos \theta & 0 \\
      0           &   0             & 1 \\
    \end{array}
  \right| = r
\]

\subparagraph{Bolcoördinaten}
\[
  \left\{
    \begin{array}{l}
      x = r \sin \theta \cos \phi\\
      y = r \sin \theta \sin \phi\\
      z = r \cos \theta \\
    \end{array}
  \right.
\]
\[
  \left| J \right| =
  \left|
    \begin{array}{ccc}
      \sin \theta \cos \phi & r \cos \theta \cos \phi & - r \sin \theta \sin \phi \\
      \sin \theta \sin \phi & r \cos \theta \sin \phi &   r \sin \theta \cos \phi \\
      \cos \theta           & - r \sin \theta         & 0 \\
    \end{array}
  \right| = r^2 \sin \theta
\]